\documentclass{article}
\usepackage{amsmath, amsfonts, fullpage}
\usepackage{amssymb}
\usepackage{graphicx}
\usepackage{hyperref}
\usepackage{algorithm}
\usepackage{algorithmic}

\title{Hubbard atom}
\author{riccardorossi0@protonmail.com}
\begin{document}
\maketitle
We consider
$$
\hat{H}=-\mu\sum_{\sigma}\hat{n}_\sigma + U\hat{n}_\uparrow \hat{n}_\downarrow
$$
One has
$$
Z = 1+2e^{\beta\mu}+e^{2\beta\mu-\beta U}
$$
and
$$
Z\,G(\tau) = -\text{Tr}\left[e^{-\beta \hat{H}}\;\psi(\tau)\;\bar{\psi}(0)\right]= -e^{\mu\tau}-e^{(\mu-U)\tau}e^{\beta\mu}
$$
One has
$$
G_{i\omega_n}=\int_0^\beta d\tau\;e^{i\omega_n\tau}G(\tau)=\frac{z_0}{i\omega_n+\mu}+\frac{z_1}{i\omega_n+\mu-U}
$$
where
$$
z_0 = \frac{1+e^{\beta\mu}}{Z}, \qquad z_0+z_1 = 1
$$
The bare propagator is
$$
G_{\text{bare},i\omega_n}=\frac{1}{i\omega_n+\mu}
$$
One has
$$
\Sigma_{i\omega_n}=\frac{z_0\,z_1\,U^2}{i\omega_n+\mu-z_0\,U}
$$
\end{document}
