\documentclass{article}
\usepackage{amsmath, amsfonts, fullpage}
\begin{document}
One has that the Chebyshev polynomial coefficients (\texttt{Coef} in the code) can be obtained as
$$
c_{k_x, k_y}:= \frac{4}{2^{n}2^m}\sum_{x=0}^{2^n -1}\, \sum_{y=0}^{2^m-1}\;f_{x,y}\;\cos\left(\frac{\pi(x+1/2)k_x}{2^n}\right)\;\cos\left(\frac{\pi(y+1/2)k_y}{2^m}\right)
$$
We define for $(k_x,k_y)\in\{0,\dots, 2^{n+1}-1\}\times\{0,\dots, 2^{m+1}-1\}$
$$
\tilde{c}_{k_x, k_y}:=e^{-\pi ik_x/2^{n+1}}e^{-\pi ik_y/2^{m+1}}\;\sum_{x=0}^{2^n-1}\sum_{y=0}^{2^m-1} f_{x,y}\;e^{-2\pi ixk_x/2^{n+1}}\;e^{-2\pi iyk_y/2^{m+1}}
$$
If we introduce for $(x, y)\in\{0,\dots,2^n-1\}\times\{0,\dots,2^m-1\}$
$$
\tilde{f}_{x,y} = f_{x,y}, \qquad \tilde{f}_{x+2^n,y} = \tilde{f}_{x,y+2^m}=\tilde{f}_{x+2^n, y+2^m} = 0
$$
one has that $\tilde{c}$ is proportional to the Fourier transform of $\tilde{f}$:
$$
\tilde{c}_{k_x, k_y}=e^{-\pi ik_x/2^{n+1}}e^{-\pi ik_y/2^{m+1}}\;\mathcal{F}[\tilde{f}](k_x, k_y)
$$
One has
$$
c_{k_x,0}=\frac{4}{2^n \,2^m}\;\text{Re}\; \tilde{c}_{k_x,0}
$$
One has for $(k_x, k_y)\in\{0,\dots, 2^n-1\}\times\{1,\dots,2^m-1\}$
$$
c_{k_x,k_y}=\frac{2}{2^n \,2^m}\left(\text{Re}\; \tilde{c}_{k_x,k_y}- \text{Re}\; \tilde{c}_{k_x,2^{m+1}-k_y}\right)
$$
\end{document}
