$$ g_{\omega_n, \omega_m, \omega_l} $$ $$
f(\tau_0, \tau_1, \tau_2, \tau_3 = 0) =
\frac{1} {
  \beta ^ 3
}
\sum_{n, m, l} g_ {
  \omega_n, \omega_m, \omega_l
}
\;
\exp\left(-i(\omega_n\tau_0+\omega_m\tau_1+\omega_l\tau_2)\right)
$$
where
$$
\omega_n := \frac{\pi(2n+1)}{\beta}
$$
and $n, m, l$ go from $-N_\omega$ to $N_\omega$.
$$
FFT((a_0, a_1, \dots, a_{N-1})=
(\sum_{n} a_n, \sum_{n} e^{2\pi i n/N} a_n,\dots,  \sum_{n} e^{2\pi i n(N-1)/N} a_n)=
(\sum_{n=0}^{N-1} e^{2\pi i kn/N} a_n)_k
$$
(we change sign of $n, l,m$)
$$
f(\tau_0, \tau_1, \tau_2, \tau_3=0)=
\frac{1}{
  \beta ^ 3}\sum_{n=-N_\omega}^{
  N_\omega}\sum_{m, l}g_{
  \omega_{-n}, \omega_{-m}, \omega_ { -l }}\;
e^{2\pi i ((n-1/2)\tau_0+(m-1/2)\tau_1+(l-1/2)\tau_2)/\beta}
$$
(we shift $n, l, m$ by $-N_\omega$)
$$
f(\tau_0, \tau_1, \tau_2, \tau_3=0)=
\frac{1}{
  \beta ^ 3}\sum_{n=0}^{
  2N_\omega}
\sum_{m=0}^{
  2N_\omega}\sum_{l=0}^{2N_\omega}
g_{
  \omega_{-n + N_\omega}, \omega_{-m + N_\omega}, \omega_ { -l + N_\omega }}\;
e^{2\pi i ((n-N_\omega-1/2)\tau_0+(m-N_\omega-1/2)\tau_1+(l-N_\omega-1/2)\tau_2)/\beta}
$$
(we take out the constant exponential factors)
$$
f(\tau_0, \tau_1, \tau_2, \tau_3=0)=
\frac{e^{
  -2\pi i(N_\omega + 1 / 2)(\tau_0 +\tau_1 +\tau_2) /\beta}}{
  \beta ^ 3}\sum_{n=0}^{
  2N_\omega}
\sum_{m=0}^{
  2N_\omega}\sum_{l=0}^{2N_\omega}
g_{
  \omega_{-n + N_\omega}, \omega_{-m + N_\omega}, \omega_ { -l + N_\omega }}\;
e^{2\pi i(n\tau_0+m\tau_1+l\tau_2)/\beta}
$$
If we choose
$$
\tau^{(k)} := \frac{\beta\,k}{2N_\omega}
$$
$$
f(\tau_0^{(k_0)}, \tau_1^{(k_1)}, \tau_2^{(k_2)})=
\frac{e^{
  -2\pi i(N_\omega + 1 / 2)(\tau_0 +\tau_1 +\tau_2) /\beta}}{
  \beta ^ 3}
\sum_{n=0}^{
  2N_\omega}\sum_{m=0}^{
  2N_\omega}\sum_{l=0}^{2N_\omega}
g_{
  \omega_{-n + N_\omega}, \omega_{-m + N_\omega}, \omega_ { -l + N_\omega }}\;
e^{2\pi i(n k_0+m k_1+l k_2)/N_\omega} 
$$
$$
f(\tau_0^{(k_0)}, \tau_1^{(k_1)}, \tau_2^{(k_2)})=
\frac{e^{
  -2\pi i /\beta(N_\omega + 1 / 2)(\tau_0 ^ {(k_0)} +\tau_1 ^ {(k_1)} +\tau_2 ^
                                   {(k_2)})}}{\beta^3} 
FFT(g_{\omega_{-n+N_\omega}, \omega_{-m+N_\omega}, \omega_{-l+N_\omega}})_k
$$
